First try for end-to-end proof

examples/fib_heap/fib_heap_panScript.sml
@@ -3,7 +3,7 @@
 *)
 Theory fib_heap_pan
 Ancestors
-  errorLogMonad panPtreeConversion panStatic set_sep address panSem fibonacci_heap
+  errorLogMonad panPtreeConversion panStatic set_sep address panSem panLang fibonacci_heap
 Libs
   stringLib numLib intLib preamble helperLib
 
@@ -19,6 +19,159 @@ in
     f (Portable.quote_to_string (fn _ => raise General.Bind) q)
 end
 
+
+(*--------------------------------------------------------
+Copied from bignum
+---------------------------------------------------------*)
+
+(** eval **********************************************************************)
+
+Theorem eval_Const[simp]:
+  eval s (Const w) = SOME (ValWord w)
+Proof
+  simp [eval_def]
+QED
+
+Theorem eval_Var_Local[simp]:
+  eval s (Var Local n) = FLOOKUP s.locals n
+Proof
+  simp [eval_def]
+QED
+
+Theorem eval_BytesInWord[simp]:
+  eval s BytesInWord = SOME (ValWord bytes_in_word)
+Proof
+  simp [eval_def]
+QED
+
+Theorem eval_Op_And_SOME:
+  eval s x₁ = SOME (ValWord v₁) ∧
+  eval s x₂ = SOME (ValWord v₂)
+  ⇒
+  eval s (Op And [x₁; x₂]) = SOME (ValWord (v₁ && v₂))
+Proof
+  simp [eval_def, wordLangTheory.word_op_def]
+QED
+
+Theorem eval_Op_Sub_SOME:
+  eval s x₁ = SOME (ValWord v₁) ∧
+  eval s x₂ = SOME (ValWord v₂)
+  ⇒
+  eval s (Op Sub [x₁; x₂]) = SOME (ValWord (v₁ - v₂))
+Proof
+  simp [eval_def, wordLangTheory.word_op_def]
+QED
+
+Theorem eval_Op_Add_SOME:
+  eval s x₁ = SOME (ValWord v₁) ∧
+  eval s x₂ = SOME (ValWord v₂)
+  ⇒
+  eval s (Op Add [x₁; x₂]) = SOME (ValWord (v₁ + v₂))
+Proof
+  simp [eval_def, wordLangTheory.word_op_def]
+QED
+
+Theorem eval_Cmp_NotEqual_SOME:
+  eval s e₁ = SOME (ValWord v₁) ∧
+  eval s e₂ = SOME (ValWord v₂)
+  ⇒
+  eval s (Cmp NotEqual e₁ e₂) = SOME (ValWord (if v₁ ≠ v₂ then 1w else 0w))
+Proof
+  simp [eval_def, asmTheory.word_cmp_def]
+QED
+
+Theorem eval_Load_One_Local_SOME:
+  FLOOKUP s.locals n = SOME (ValWord v) ∧
+  v ∈ s.memaddrs
+  ⇒
+  eval s (Load One (Var Local n)) = SOME (Val (s.memory v))
+Proof
+  simp [eval_def, mem_load_def]
+QED
+
+(** evaluate ******************************************************************)
+
+Theorem evaluate_Annot[simp]:
+  evaluate (Annot s₁ s₂, s) = (NONE, s)
+Proof
+  simp [evaluate_def]
+QED
+
+Theorem evaluate_Seq_Annot[simp]:
+  evaluate (Seq (Annot s₁ s₂) c, s) = evaluate (c, s) ∧
+  evaluate (Seq c (Annot s₁ s₂), s) = evaluate (c, s)
+Proof
+  simp [evaluate_def]
+  >> rpt (pairarg_tac >> gvs [])
+  >> IF_CASES_TAC >> simp []
+QED
+
+Theorem evaluate_Seq_assoc[simp]:
+  evaluate (Seq (Seq s₁ s₂) (Seq s₃ s₄), s) =
+  evaluate (Seq s₁ (Seq s₂ (Seq s₃ s₄)), s)
+Proof
+  simp [evaluate_def]
+  >> rpt (pairarg_tac >> gvs [])
+  >> rpt (IF_CASES_TAC >> gvs [])
+QED
+
+Theorem evaluate_While_True_NONE:
+  eval s e = SOME (ValWord w) ∧ w ≠ 0w ∧ s.clock ≠ 0 ∧
+  evaluate (c, dec_clock s) = (NONE, s₁) ∧
+  evaluate (While e c, s₁) = (NONE, s')
+  ⇒
+  evaluate (While e c,s) = (NONE, s')
+Proof
+  rw [] >> simp [Once evaluate_def]
+QED
+
+
+
+Theorem evaluate_Dec_NONE:
+  eval s e = SOME value ∧
+  evaluate (prog,s with locals := s.locals |+ (v,value)) = (NONE,s₁)
+  ⇒
+  evaluate (Dec v shape e prog, s) =
+    (NONE, s₁ with locals := res_var s₁.locals (v, FLOOKUP s.locals v))
+Proof
+  rw [] >> simp [Once evaluate_def]
+QED
+
+Theorem evaluate_Seq_NONE:
+  evaluate (c₁, s) = (NONE, s₁) ∧
+  evaluate (c₂, s₁) = (NONE, s')
+  ⇒
+  evaluate (Seq c₁ c₂, s) = (NONE, s')
+Proof
+  rw [] >> simp [evaluate_def]
+QED
+
+Theorem evaluate_Store_Local_NONE:
+  FLOOKUP s.locals dst = SOME (ValWord addr) ∧
+  addr ∈ s.memaddrs ∧
+  eval s e = SOME (Val v)
+  ⇒
+  evaluate (Store (Var Local dst) e, s) =
+    (NONE, s with memory := s.memory⦇addr ↦ v⦈)
+Proof
+  simp [evaluate_def, flatten_def, mem_stores_def, mem_store_def]
+QED
+
+Theorem evaluate_Assign_Local:
+  eval s src = SOME value ∧
+  FLOOKUP s.locals dst = SOME old_value ∧
+  shape_of value = shape_of old_value
+  ⇒
+  evaluate ((Assign Local dst src), s) = (NONE, set_var dst value s)
+Proof
+  simp [evaluate_def, is_valid_value_def]
+QED
+
+
+(*----------------------------------------------------------
+ Pancake code
+-----------------------------------------------------------*)
+
 (** Copied from panPtreeConversion *)
 fun parse_pancake q =
   let
@@ -28,18 +181,38 @@ fun parse_pancake q =
   end
 
 
-Quote melt_pan = parse_pancake:
-  fun 1 melt (1 a1, 1 a2) {
-    if (a2 == 0) {return a1;} else {}
-    if (a1 == 0) {return a2;} else {}
-    return a1;
+Quote meld_pan = parse_pancake:
+  fun meld (a1,a2) {
+    if (a2 == 0) {
+      return a1;
+    }
+    if (a1 == 0) {
+      return a2;
+    }
+
+    var l_a1 = lds 1 (a1 + 4);
+    var l_a2 = lds 1 (a2 + 4);
+
+    st l_a1 + 5, a2;
+    st a2   + 4, l_a1;
+    st l_a2 + 5, a1;
+    st a1   + 4, l_a2;
+
+    var v1 = lds 1 a1;
+    var v2 = lds 1 a2;
+
+    if v1 <= v2 {
+        return a1;
+    } else {
+        return a2;
+    }
   }
 End
 
 
-Definition melt_body_def:
-  melt_body =
-    ^(find_term (can $ match_term “panLang$Seq _ _”) melt_pan)
+Definition meld_body_def:
+  meld_body =
+    ^(find_term (can $ match_term “panLang$Seq _ _”) meld_pan)
 End
 
 
@@ -55,6 +228,7 @@ Theorem evaluate_Annot[simp]:
 Proof
   simp [evaluate_def]
 QED
+
 
 Theorem evaluate_Seq_Annot[simp]:
   evaluate (Seq (Annot s₁ s₂) c, s) = evaluate (c, s) ∧
@@ -140,18 +314,34 @@ QED
 *)
 
 
-Theorem melt_pan_thm:
+Theorem meld_pan_thm:
   ∀a1 a2 dm m frame s.
-    fib_heap_melt (a1,a2,m,dm) = (a',m',T) /\
+    fib_heap_meld (a1,a2,m,dm) = (a',m',T) /\
     FLOOKUP s.locals (strlit "a1") = SOME (Val (Word a1)) ∧
     FLOOKUP s.locals (strlit "a2") = SOME (Val (Word a2)) ∧
     m = s.memory /\ dm = s.memaddrs
     ⇒
     ∃l.
-      evaluate (melt_body,s) = (NONE,
+      evaluate (meld_body,s) = (SOME (Return (ValWord a')),
         s with <| memory := m';
                   locals := l |>)
 Proof
+  rpt strip_tac >>
+  rw[fib_heap_meld_def] >>
+  simp[meld_body_def] >>
+  simp[Once evaluate_def] >>
+(**)
+  pairarg_tac >> simp[] >> pop_assum mp_tac >>
+  simp[Once evaluate_def,eval_def,asmTheory.word_cmp_def] >>
+  CASE_TAC >> simp[]
+  >- (
+    simp[Once evaluate_def] >>
+    simp[shape_of_def,size_of_shape_def] >>
+    strip_tac >> gvs[] >>
+    fs[fib_heap_meld_def] >>
+    qexists `FEMPTY` >> simp[empty_locals_def,state_component_equality]
+    ) >>
+  simp[Once evaluate_def] >> strip_tac >> gvs[] >>
   cheat
 QED
 
